coq/Extra.v
@@ -1,6 +1,6 @@
 From mathcomp Require Import
   ssreflect ssrfun ssrbool ssrnat eqtype seq choice fintype path
-  ssrint rat.
+  ssrint rat bigop.
 
 From extructures Require Import ord fset fmap ffun.
 
@@ -11,6 +11,66 @@ Unset Printing Implicit Defensive.
 Local Open Scope fset_scope.
 
 (* Consolidate this stuff in extructures. *)
+
+Lemma fmap_ind (T : ordType) S (P : {fmap T -> S} -> Prop) :
+  P emptym ->
+  (forall m, P m -> forall x y, x \notin domm m -> P (setm m x y)) ->
+  forall m, P m.
+Proof.
+move=> H0 H1 m; move e: (domm m)=> X.
+elim/fset_ind: X m e=> [|x X x_X IH] m e.
+  by move/eqP/emptymP: e=> ->.
+have /dommP [y yP]: x \in domm m by rewrite e in_fsetU1 eqxx.
+set m' := remm m x; have em : m = setm m' x y.
+  apply/eq_fmap=> x'; rewrite /m' setmE remmE.
+  by case: eqP => [->|].
+have {}e : domm m' = X.
+  apply/eq_fset=> x'; rewrite /m' domm_rem e in_fsetD1 in_fsetU1.
+  by case: eqP=> // -> /=; rewrite (negbTE x_X).
+rewrite {}em; apply: H1; first by exact: IH.
+by rewrite e.
+Qed.
+
+Lemma remmI (T : ordType) S (m : {fmap T -> S}) x :
+  x \notin domm m ->
+  remm m x = m.
+Proof.
+move=> /dommPn m_x; apply/eq_fmap=> x'; rewrite remmE.
+by case: eqP=> // ->; rewrite m_x.
+Qed.
+
+Lemma setm_rem (T : ordType) S m (x : T) (y : S) :
+  setm (remm m x) x y = setm m x y.
+Proof.
+apply/eq_fmap=> x'; rewrite !setmE !remmE.
+by case: eqP.
+Qed.
+
+Lemma eq_setm (T : ordType) (S : eqType) m1 m2 (x : T) (y1 y2 : S) :
+  (setm m1 x y1 == setm m2 x y2) =
+  (y1 == y2) && (remm m1 x == remm m2 x).
+Proof.
+apply/(sameP eqP)/(iffP andP).
+  rewrite -[setm m1 x y1]setm_rem.
+  by case=> /eqP -> /eqP ->; rewrite setm_rem.
+move=> /eq_fmap e.
+move: (e x); rewrite !setmE eqxx; case=> ->; split=> //.
+apply/eqP/eq_fmap=> x'; move: (e x'); rewrite !setmE !remmE.
+by case: eqP.
+Qed.
+
+Lemma big_fsetU1 R (idx : R) (op : Monoid.com_law idx) (I : ordType) (x : I) (X : {fset I}) (P : pred I) (F : I -> R) :
+  x \notin X ->
+  let y := \big[op/idx]_(i <- X | P i) F i in
+  \big[op/idx]_(i <- x |: X | P i) F i =
+  if P x then op (F x) y else y.
+Proof.
+move=> x_X.
+have e: perm_eq (x |: X) (x :: X).
+  apply: uniq_perm; rewrite /= ?x_X ?uniq_fset // => x'.
+  by rewrite inE in_fsetU1.
+by rewrite /= (perm_big _ e) big_cons.
+Qed.
 
 Lemma val_fset_filter (T : ordType) (P : T -> bool) (X : {fset T}) :
   fset_filter P X = filter P X :> seq T.
@@ -114,6 +174,54 @@ Proof.
 by apply/eq_fmap=> x; rewrite !mapmE !mkfmapfE /=; case: ifP.
 Qed.
 
+Section SetSplitting.
+
+Variables (T : ordType).
+
+Implicit Types X : {fset T}.
+
+Definition splits X :=
+  if val X is x :: xs then Some (x, fset xs)
+  else None.
+
+End SetSplitting.
+
+Section MapSplitting.
+
+Variables (T : ordType) (S : Type).
+Implicit Types m : {fmap T -> S}.
+
+Definition splitm m :=
+  match val m with
+  | (x, y) :: ps => Some (x, y, mkfmap ps)
+  | [::] => None
+  end.
+
+Lemma sizeES m :
+  size m = if splitm m is Some (_, _, m') then (size m').+1 else 0.
+Proof.
+rewrite /splitm /=; move: (valP m)=> /=.
+by case: (val m)=> [|[x y] m'] //= /path_sorted /mkfmapK ->.
+Qed.
+
+Lemma domm_mkfmap' (ps : seq (T * S)) :
+  domm (mkfmap ps) = fset (unzip1 ps).
+Proof.
+by apply/eq_fset=> x; rewrite domm_mkfmap in_fset.
+Qed.
+
+Lemma dommES m :
+  domm m = if splitm m is Some (x, _, m) then x |: domm m
+           else fset0.
+Proof.
+rewrite /domm /splitm /=.
+case: m=> [[|[x y] m] mP] //=; first by rewrite fset0E.
+move: mP=> /= /path_sorted/mkfmapK ->.
+by rewrite fset_cons.
+Qed.
+
+End MapSplitting.
+
 Section Update.
 
 Context {T : ordType} {S : eqType} {def : T -> S}.
@@ -142,3 +250,65 @@ by rewrite /mkffunm mkffunE mem_domm; case: (m x).
 Qed.
 
 Arguments fdisjointP {_ _ _}.
+
+Definition mapf (T : ordType) (S R : eqType) (def : T -> S) (g : S -> R) (f : ffun def) : ffun (g \o def) :=
+  mkffun (g \o f) (supp f).
+
+Lemma mapfE (T : ordType) (S R : eqType) (def : T -> S) (g : S -> R) (f : ffun def) x :
+  mapf g f x = g (f x).
+Proof.
+rewrite /mapf mkffunE mem_supp /=.
+by case: eqP=> //= ->.
+Qed.
+
+Lemma val_mkffun (T : ordType) (S : eqType) (def : T -> S) (f : T -> S) (X : {fset T}) :
+  @ffval _ _ def (mkffun f X) =
+  mkfmapfp (fun x => if f x == def x then None else Some (f x)) X.
+Proof.
+apply/eq_fmap=> x; rewrite mkfmapfpE.
+move: (@mkffunE _ _ def f X x); rewrite /appf /=.
+set ff := mkffun f X; case e: (ffval ff x) => [y|].
+- have xdomm: x \in domm (ffval ff) by rewrite mem_domm e.
+  move/allP/(_ _ xdomm): (valP ff); rewrite /= e => yP ey.
+  move: yP; rewrite {}ey; case: ifP; last by rewrite eqxx.
+  rewrite inj_eq; last exact: Some_inj.
+  by move=> _ /negbTE ->.
+- by case: ifP=> // _ ->; rewrite eqxx.
+Qed.
+
+Lemma val_mapf (T : ordType) (S R : eqType) (def : T -> S) (g : S -> R) :
+  injective g ->
+  forall f : ffun def, ffval (mapf g f) = mapm g (ffval f).
+Proof.
+move=> g_inj f; apply/eq_fmap=> x.
+rewrite /mapf val_mkffun mkfmapfpE mapmE mem_supp /= /appf /=.
+rewrite inj_eq //.
+case e: (ffval f x)=> [y|] /=; last by rewrite eqxx.
+have xdomm: x \in domm (ffval f) by rewrite mem_domm e.
+move/allP/(_ _ xdomm): (valP f); rewrite e.
+rewrite inj_eq; last exact: Some_inj.
+by move=> /negbTE ->.
+Qed.
+
+Lemma fset1_inj (T : ordType) : injective (@fset1 T).
+Proof.
+by move=> x y e; apply/fset1P; rewrite -e; apply/fset1P.
+Qed.
+
+Definition pimfset (T S : ordType) (f : T -> option S) (X : {fset T}) : {fset S} :=
+  fset (pmap f X).
+
+Lemma in_pimfset (T S : ordType) (f : T -> option S) (X : {fset T}) y :
+  y \in (pimfset f X) = (Some y \in f @: X).
+Proof.
+rewrite /pimfset in_fset mem_pmap.
+by apply/(sameP mapP)/(iffP imfsetP).
+Qed.
+
+Lemma pimfsetP (T S : ordType) (f : T -> option S) (X : {fset T}) y :
+  reflect (exists2 x, x \in X & f x = Some y) (y \in pimfset f X).
+Proof.
+rewrite in_pimfset; apply/(iffP imfsetP); case=> ??.
+- by move=> ->; eauto.
+- by move=> <-; eauto.
+Qed.
